calling aead from hashaccumulator

steel/Zeta.Steel.HashAccumulator.fst
@@ -5,14 +5,28 @@ module U64 = FStar.UInt64
 module Cast = FStar.Int.Cast
 module A = Steel.ST.Array
 open Steel.ST.Util
-module Blake = Hacl.Blake2b_32
+module AEAD = EverCrypt.AEAD
 module Loops = Steel.ST.Loops
 module R = Steel.ST.Reference
 module G = Zeta.Steel.Globals
 #push-options "--ide_id_info_off"
 #push-options "--fuel 0 --ifuel 0"
 
-let hash_value_buf  = x:A.array U8.t { A.length x == 32 /\ A.is_full_array x }
+let hash_len_sz = 16sz
+let hash_len = SizeT.v hash_len_sz
+let hash_value_t =
+    Ghost.erased (Seq.lseq U8.t hash_len &
+                  nat)
+let hash_of (h:hash_value_t)
+  : GTot (Seq.lseq U8.t hash_len)
+  = fst h
+
+let ctr_of (h:hash_value_t)
+  : GTot nat
+  = snd h
+
+let hash_value_buf  = x:A.array U8.t { A.length x == hash_len /\ A.is_full_array x }
+
 
 //[@@CAbstractStruct] TODO: Restore this after krml #247
 noeq
@@ -22,41 +36,42 @@ type ha = {
   tmp: hash_value_buf
 }
 
+
 // [@@__steel_reduce__;__reduce__]
-let ha_val (h:ha) (s:ehash_value_t) =
-  A.pts_to h.acc full_perm (fst s) `star`
+let ha_val (h:ha) (s:hash_value_t) =
+  A.pts_to h.acc full_perm (hash_of s) `star`
   exists_ (fun (n:U32.t) ->
-      pure (U32.v n == snd s) `star`
+      pure (U32.v n == ctr_of s) `star`
       R.pts_to h.ctr full_perm n) `star`
   exists_ (A.pts_to h.tmp full_perm)
       
-let unfold_ha_val (#o:_) (h:ha) (s:ehash_value_t)
+let unfold_ha_val (#o:_) (h:ha) (s:hash_value_t)
   : STGhostT unit o
     (ha_val h s)
-    (fun _ -> A.pts_to h.acc full_perm (fst s) `star`
+    (fun _ -> A.pts_to h.acc full_perm (hash_of s) `star`
            exists_ (fun (n:U32.t) ->
-             pure (U32.v n == snd s) `star`
+             pure (U32.v n == ctr_of s) `star`
              R.pts_to h.ctr full_perm n) `star`
            exists_ (A.pts_to h.tmp full_perm))
   = rewrite (ha_val h s)
-            (A.pts_to h.acc full_perm (fst s) `star`
+            (A.pts_to h.acc full_perm (hash_of s) `star`
              exists_ (fun (n:U32.t) ->
-                pure (U32.v n == snd s) `star`
+                pure (U32.v n == ctr_of s) `star`
                 R.pts_to h.ctr full_perm n) `star`
              exists_ (A.pts_to h.tmp full_perm));
     ()
 
-let fold_ha_val (#o:_) (h:ha) (s:ehash_value_t)
+let fold_ha_val (#o:_) (h:ha) (s:hash_value_t)
   : STGhostT unit o
-    (A.pts_to h.acc full_perm (fst s) `star`
+    (A.pts_to h.acc full_perm (hash_of s) `star`
      exists_ (fun (n:U32.t) ->
-       pure (U32.v n == snd s) `star`
+       pure (U32.v n == ctr_of s) `star`
        R.pts_to h.ctr full_perm n)  `star`
      exists_ (A.pts_to h.tmp full_perm))
     (fun _ -> ha_val h s)
-  = rewrite (A.pts_to h.acc full_perm (fst s) `star`
+  = rewrite (A.pts_to h.acc full_perm (hash_of s) `star`
              exists_ (fun (n:U32.t) ->
-               pure (U32.v n == snd s) `star`
+               pure (U32.v n == ctr_of s) `star`
                R.pts_to h.ctr full_perm n) `star`
              exists_ (A.pts_to h.tmp full_perm))
             (ha_val h s);
@@ -64,13 +79,13 @@ let fold_ha_val (#o:_) (h:ha) (s:ehash_value_t)
 
 
 let initial_hash
-  = Seq.create 32 0uy, 0
+  = Ghost.hide (Seq.create hash_len 0uy, 0)
 
 let hash_one_value 
       (iv:Seq.seq U8.t { Seq.length iv == iv_len })
-      (s:Seq.seq U8.t { Seq.length s <= blake2_max_input_length })
+      (s:Seq.seq U8.t { Seq.length s <= aead_max_input_length })
   : hash_value_t
-  = Blake.spec s 0 Seq.empty 32, 1
+  = AEAD.spec G.aead_key iv s, 1
 
 noextract inline_for_extraction
 let xor_bytes (s1: Seq.seq U8.t)
@@ -118,8 +133,8 @@ let xor_bytes_associative
 
 let aggregate_hashes (h0 h1: hash_value_t)
   : hash_value_t
-  = xor_bytes (fst h0) (fst h1),
-    snd h0 + snd h1
+  = xor_bytes (hash_of h0) (hash_of h1),
+    ctr_of h0 + ctr_of h1
 
 let initial_hash_unit h = xor_bytes_unit (fst h)
 
@@ -129,15 +144,15 @@ let aggregate_hashes_commutative h1 h2 =
 let aggregate_hashes_associative h1 h2 h3 =
   xor_bytes_associative (fst h1) (fst h2) (fst h3)
 
-let mk_hash_value (ws:Seq.lseq U8.t 32) (wc:U32.t)
+let mk_hash_value (ws:Seq.lseq U8.t hash_len) (wc:U32.t)
   : hash_value_t
   = ws, U32.v wc
 
 let intro_ha_val (#o:_)
                  (s:ha)
-                 (ws:Seq.lseq U8.t 32)
+                 (ws:Seq.lseq U8.t hash_len)
                  (wc:U32.t)
-                 (res:Ghost.erased hash_value_t { Ghost.reveal res == mk_hash_value ws wc })
+                 (res:hash_value_t { res == mk_hash_value ws wc })
   : STGhostT unit o
     (A.pts_to s.acc full_perm ws
       `star`
@@ -157,7 +172,7 @@ let intro_ha_val (#o:_)
     ()
 
 
-let elim_ha_val #o (#w:ehash_value_t) (s:ha)
+let elim_ha_val #o (#w:hash_value_t) (s:ha)
   : STGhost (Ghost.erased U32.t) o
     (ha_val s w)
     (fun n -> A.pts_to s.acc full_perm (fst w) `star`
@@ -171,22 +186,22 @@ let elim_ha_val #o (#w:ehash_value_t) (s:ha)
     n
 
 let create (_:unit)
-  = let acc = A.alloc 0uy 32sz in
+  = let acc = A.alloc 0uy hash_len_sz in
     let ctr = R.alloc 0ul in
-    let tmp = A.alloc 0uy 32sz in
+    let tmp = A.alloc 0uy hash_len_sz in
     let ha = { acc; ctr; tmp } in
     //TODO: constructing values and transporting slprops to their fields is very tedious
     rewrite (A.pts_to acc _ _)
-            (A.pts_to ha.acc full_perm (Seq.create 32 0uy));
+            (A.pts_to ha.acc full_perm (Seq.create hash_len 0uy));
     rewrite (R.pts_to ctr _ _)
             (R.pts_to ha.ctr full_perm 0ul);
     rewrite (A.pts_to tmp _ _)
-            (A.pts_to ha.tmp full_perm (Seq.create 32 0uy));
+            (A.pts_to ha.tmp full_perm (Seq.create hash_len 0uy));
     intro_exists _ (A.pts_to ha.tmp full_perm);
     intro_ha_val ha _ _ initial_hash;
     return ha
 
-let reclaim (#h:ehash_value_t) (s:ha)
+let reclaim (#h:hash_value_t) (s:ha)
   = let _ = elim_ha_val s in
     R.free s.ctr;
     A.free s.tmp;    
@@ -206,7 +221,7 @@ let xor_bytes_pfx (s1:bytes)
 
 let raw_hash_t = Seq.seq U8.t
 
-let eraw_hash_t = s:Ghost.erased raw_hash_t { Seq.length s == 32 }
+let eraw_hash_t = s:Ghost.erased raw_hash_t { Seq.length s == hash_len }
 
 let extend_hash_value (s1 s2:bytes)
                       (i:nat)
@@ -230,7 +245,7 @@ let aggregate_raw_hashes
     (fun _ ->
      A.pts_to b1 full_perm (xor_bytes s1 s2) `star`
      A.pts_to b2 full_perm s2)
-  = let inv (i:Loops.nat_at_most 32sz)
+  = let inv (i:Loops.nat_at_most hash_len_sz)
       : vprop
       = A.pts_to b1 full_perm (xor_bytes_pfx s1 s2 i) `star`
         A.pts_to b2 full_perm s2
@@ -238,7 +253,7 @@ let aggregate_raw_hashes
     A.pts_to_length b1 _;
     A.pts_to_length b2 _;
     [@@inline_let]
-    let body (i:Loops.u32_between 0sz 32sz)
+    let body (i:Loops.u32_between 0sz hash_len_sz)
       : STT unit
         (inv (SizeT.v i))
         (fun _ -> inv (SizeT.v i + 1))
@@ -263,9 +278,9 @@ let aggregate_raw_hashes
     assert (xor_bytes_pfx s1 s2 0 `Seq.equal` s1);
     rewrite (A.pts_to b1 _ _ `star` A.pts_to b2 _ _)
             (inv 0);
-    Loops.for_loop 0sz 32sz inv body;
-    assert (xor_bytes_pfx s1 s2 32 `Seq.equal` xor_bytes s1 s2);
-    rewrite (inv 32)
+    Loops.for_loop 0sz hash_len_sz inv body;
+    assert (xor_bytes_pfx s1 s2 hash_len `Seq.equal` xor_bytes s1 s2);
+    rewrite (inv hash_len)
             (A.pts_to b1 _ _ `star` A.pts_to b2 _ _);
     return ()
 
@@ -281,47 +296,47 @@ type ha_core = {
   ctr:R.ref U32.t;
 }
 
-let ha_core_val (h:ha_core) (s:ehash_value_t) =
-  A.pts_to h.acc full_perm (fst s) `star`
+let ha_core_val (h:ha_core) (s:hash_value_t) =
+  A.pts_to h.acc full_perm (hash_of s) `star`
   exists_ (fun (n:U32.t) ->
-      pure (U32.v n == snd s) `star`
+      pure (U32.v n == ctr_of s) `star`
       R.pts_to h.ctr full_perm n)
 
-let elim_ha_core_val #o (#s:ehash_value_t) (h:ha_core)
+let elim_ha_core_val #o (#s:hash_value_t) (h:ha_core)
   : STGhost (Ghost.erased U32.t) o
     (ha_core_val h s)
-    (fun n -> A.pts_to h.acc full_perm (fst s) `star`
+    (fun n -> A.pts_to h.acc full_perm (hash_of s) `star`
            R.pts_to h.ctr full_perm n)
     (requires True)
     (ensures fun n -> U32.v n == snd s)
   = rewrite (ha_core_val h s)
-            (A.pts_to h.acc full_perm (fst s) `star`
+            (A.pts_to h.acc full_perm (hash_of s) `star`
              exists_ (fun (n:U32.t) ->
-               pure (U32.v n == snd s) `star`
+               pure (U32.v n == ctr_of s) `star`
                R.pts_to h.ctr full_perm n));
     let n = elim_exists () in
     elim_pure _;
     n
 
-let fold_ha_core_val (#o:_) (h:ha_core) (s:ehash_value_t)
+let fold_ha_core_val (#o:_) (h:ha_core) (s:hash_value_t)
   : STGhostT unit o
-    (A.pts_to h.acc full_perm (fst s) `star`
+    (A.pts_to h.acc full_perm (hash_of s) `star`
      exists_ (fun (n:U32.t) ->
-       pure (U32.v n == snd s) `star`
+       pure (U32.v n == ctr_of s) `star`
        R.pts_to h.ctr full_perm n))
     (fun _ -> ha_core_val h s)
-  = rewrite (A.pts_to h.acc full_perm (fst s) `star`
+  = rewrite (A.pts_to h.acc full_perm (hash_of s) `star`
              exists_ (fun (n:U32.t) ->
-               pure (U32.v n == snd s) `star`
+               pure (U32.v n == ctr_of s) `star`
                R.pts_to h.ctr full_perm n))
             (ha_core_val h s);
     ()
 
 let intro_ha_core_val (#o:_)
                       (s:ha_core)
-                      (ws:Seq.lseq U8.t 32)
+                      (ws:Seq.lseq U8.t hash_len)
                       (wc:U32.t)
-                      (res:Ghost.erased hash_value_t { Ghost.reveal res == mk_hash_value ws wc })
+                      (res:hash_value_t { res == mk_hash_value ws wc })
   : STGhostT unit o
     (A.pts_to s.acc full_perm ws
       `star`
@@ -330,15 +345,15 @@ let intro_ha_core_val (#o:_)
       ha_core_val s res)
   = let w = mk_hash_value ws wc in
     rewrite (A.pts_to s.acc _ _)
-            (A.pts_to s.acc full_perm (fst w));
-    intro_pure (U32.v wc == snd w);
-    intro_exists #U32.t wc (fun n -> pure (U32.v n == snd w) `star` R.pts_to s.ctr full_perm n);
+            (A.pts_to s.acc full_perm (hash_of w));
+    intro_pure (U32.v wc == ctr_of w);
+    intro_exists #U32.t wc (fun n -> pure (U32.v n == ctr_of w) `star` R.pts_to s.ctr full_perm n);
     fold_ha_core_val s w;
     rewrite (ha_core_val s w)
             (ha_core_val s res);
     ()
 
-let aggregate_core (#h1 #h2:ehash_value_t) (b1 b2: ha_core)
+let aggregate_core (#h1 #h2:hash_value_t) (b1 b2: ha_core)
   : STT bool
     (ha_core_val b1 h1 `star` ha_core_val b2 h2)
     (fun b -> ha_core_val b1 (maybe_aggregate_hashes b h1 h2) `star` ha_core_val b2 h2)
@@ -366,7 +381,7 @@ let aggregate_core (#h1 #h2:ehash_value_t) (b1 b2: ha_core)
       return true
     )
 
-let ha_val_as_core_val #o (#w:ehash_value_t) (b:ha)
+let ha_val_as_core_val #o (#w:hash_value_t) (b:ha)
   : STGhostT unit o
     (ha_val b w)
     (fun r -> ha_core_val {acc=b.acc; ctr=b.ctr} w `star`
@@ -374,7 +389,7 @@ let ha_val_as_core_val #o (#w:ehash_value_t) (b:ha)
   = let c = elim_ha_val b in
     intro_ha_core_val {acc=b.acc; ctr=b.ctr} _ _ w
 
-let ha_core_val_as_ha_val #o (#w:ehash_value_t) (b:ha_core) (tmp:hash_value_buf)
+let ha_core_val_as_ha_val #o (#w:hash_value_t) (b:ha_core) (tmp:hash_value_buf)
   : STGhostT unit o
     (ha_core_val b w `star` exists_ (A.pts_to tmp full_perm))
     (fun r -> ha_val {acc=b.acc; ctr=b.ctr; tmp} w)
@@ -408,13 +423,52 @@ let compare #h1 #h2 (b1 b2:ha)
       return false
     )
     else (
-      let b = Steel.ST.Array.Util.compare b1.acc b2.acc 32sz in
+      let b = Steel.ST.Array.Util.compare b1.acc b2.acc hash_len_sz in
       assert (b <==> (fst h1 == fst h2));
       intro_ha_val b1 _ _ h1;
       intro_ha_val b2 _ _ h2;
       return b
     )
 
+let get_aead_key (#o:_) (_:unit)
+  : STGhostT perm o
+      emp
+      (fun p -> A.pts_to G.aead_key_buffer p G.aead_key)
+  = admit_(); full_perm
+
+let aead_with_key  
+         (#iv_p:perm)
+         (#iv_v:Ghost.erased (Seq.seq U8.t) { Seq.length iv_v == iv_len })
+         (iv: A.array U8.t)
+         (#in_p:perm)         
+         (#in_v:Ghost.erased (Seq.seq U8.t))
+         (input:hashable_buffer)
+         (input_len:U32.t { U32.v input_len == Seq.length in_v /\
+                            A.length input == Seq.length in_v })
+         (out:hash_value_buf)
+  : STT AEAD.error_code
+    (A.pts_to iv iv_p iv_v `star`
+     A.pts_to input in_p in_v `star`
+     exists_ (A.pts_to out full_perm))
+    (fun res -> 
+     A.pts_to iv iv_p iv_v `star`
+     A.pts_to input in_p in_v `star`
+     exists_ (fun out_v -> 
+       A.pts_to out full_perm out_v `star`
+       pure (res == 0uy ==> out_v == AEAD.spec G.aead_key iv_v in_v)))
+  = let k_p = get_aead_key () in
+    let res =
+      AEAD.encrypt_expand_aes128_gcm_no_check
+           G.aead_key_buffer
+           iv 96ul
+           input input_len
+           R.null 0ul
+           R.null
+           out in
+    drop (A.pts_to G.aead_key_buffer _ _);
+    return res
+
+#push-options "--query_stats --z3rlimit_factor 4"
 let add #h (ha:ha)
         #p #ivv
         #s
@@ -423,33 +477,44 @@ let add #h (ha:ha)
         l
   = R.with_local 1ul (fun ctr ->
      ha_val_as_core_val ha;                 
-     let _out = elim_exists () in
-     let _dummy = A.alloc 0uy 1sz in //TODO: Really should  R.null, but kremlin doesn't handle that yet
-     Blake.blake2b 32ul ha.tmp l input 0ul _dummy;
-     let ha_core' = { acc=ha.tmp; ctr } in
-     rewrite (A.pts_to ha.tmp _ _)
-             (A.pts_to ha_core'.acc full_perm
+     assume (U32.v l == A.length input);
+     let success = aead_with_key iv input l ha.tmp in
+     let out_ = elim_exists () in
+     elim_pure _;
+     if success <> 0uy
+     then (
+      intro_exists_erased out_ (A.pts_to ha.tmp full_perm);
+      ha_core_val_as_ha_val {acc=ha.acc; ctr=ha.ctr} ha.tmp;
+      rewrite (ha_val {acc=ha.acc; ctr=ha.ctr; tmp=ha.tmp} _)
+              (ha_val ha (maybe_aggregate_hashes false h
+                                                  (hash_one_value ivv (Seq.slice s 0 (U32.v l)))));
+      return false
+     )
+     else (
+       let ha_core' = { acc=ha.tmp; ctr } in
+       rewrite (A.pts_to ha.tmp _ _)
+               (A.pts_to ha_core'.acc full_perm
                        (fst (hash_one_value ivv (Seq.slice s 0 (U32.v l)))));
-     rewrite (R.pts_to ctr _ _)
-             (R.pts_to ha_core'.ctr full_perm 1ul);
-     //TODO: marking ha_val steel_reduce leads to a failure here
-     intro_ha_core_val ha_core' 
-                       (fst (hash_one_value ivv (Seq.slice s 0 (U32.v l))))
-                       1ul
-                       (hash_one_value ivv (Seq.slice s 0 (U32.v l)));
-     let b = aggregate_core {acc=ha.acc; ctr=ha.ctr} ha_core' in
-     let n = elim_ha_core_val ha_core' in
-     rewrite (R.pts_to ha_core'.ctr full_perm n)
-             (R.pts_to ctr full_perm n);
-     rewrite (A.pts_to ha_core'.acc _ _)
-             (A.pts_to ha.tmp full_perm 
-                       (fst (hash_one_value ivv (Seq.slice s 0 (U32.v l)))));
-     intro_exists _ (A.pts_to ha.tmp full_perm);
-     ha_core_val_as_ha_val {acc=ha.acc; ctr=ha.ctr} ha.tmp;
-     rewrite (ha_val {acc=ha.acc; ctr=ha.ctr; tmp=ha.tmp} _)
-             (ha_val ha (maybe_aggregate_hashes b h
-                          (hash_one_value ivv (Seq.slice s 0 (U32.v l)))));
-     intro_exists _ (A.pts_to _dummy full_perm);
-     A.free _dummy;
-     return b)
-
+       rewrite (R.pts_to ctr _ _)
+               (R.pts_to ha_core'.ctr full_perm 1ul);
+       //TODO: marking ha_val steel_reduce leads to a failure here
+       intro_ha_core_val ha_core' 
+                         (fst (hash_one_value ivv (Seq.slice s 0 (U32.v l))))
+                         1ul
+                         (hash_one_value ivv (Seq.slice s 0 (U32.v l)));
+       let b = aggregate_core {acc=ha.acc; ctr=ha.ctr} ha_core' in
+       let n = elim_ha_core_val ha_core' in
+       rewrite (R.pts_to ha_core'.ctr full_perm n)
+               (R.pts_to ctr full_perm n);
+       rewrite (A.pts_to ha_core'.acc _ _)
+               (A.pts_to ha.tmp full_perm 
+                         (fst (hash_one_value ivv (Seq.slice s 0 (U32.v l)))));
+       intro_exists _ (A.pts_to ha.tmp full_perm);
+       ha_core_val_as_ha_val {acc=ha.acc; ctr=ha.ctr} ha.tmp;
+       rewrite (ha_val {acc=ha.acc; ctr=ha.ctr; tmp=ha.tmp} _)
+               (ha_val ha (maybe_aggregate_hashes b h
+                                                  (hash_one_value ivv (Seq.slice s 0 (U32.v l)))));
+       return b
+     )
+    )
+#pop-options
