steel/Zeta.Steel.HashAccumulator.fsti
@@ -5,29 +5,26 @@ module A = Steel.ST.Array
 open Steel.ST.Util
 
 inline_for_extraction noextract
-let blake2_max_input_length = pow2 32 - 1 - 128
+let aead_max_input_length = pow2 31
 
 // NOTE: we do not have an agile spec for the keyed hash functionality :(, so
 // we're making Blake2-dependent assumptions without corresponding agile predicates
 noextract inline_for_extraction
-let hashable_bytes = s:Seq.seq U8.t { Seq.length s <= blake2_max_input_length }
-let hashable_buffer = b:A.array U8.t { A.length b <= blake2_max_input_length }
+let hashable_bytes = s:Seq.seq U8.t { Seq.length s < aead_max_input_length }
+let hashable_buffer = b:A.array U8.t { A.length b < aead_max_input_length }
 
+inline_for_extraction noextract
 let iv_len = 96
 let iv_t = Seq.lseq U8.t iv_len
 let iv_buffer = b:A.array U8.t { A.length b == iv_len }
 
-let hash_len = 32
-let hash_value_t = 
-  Seq.lseq U8.t hash_len &
-  nat
-  
-let ehash_value_t = Ghost.erased hash_value_t
+[@@erasable]
+val hash_value_t : Type0
 
 val ha
   : Type0
 
-val ha_val (r:ha) (v:ehash_value_t)
+val ha_val (r:ha) (v:hash_value_t)
   : vprop
   
 val initial_hash
@@ -58,7 +55,7 @@ val create (_:unit)
     (fun s -> ha_val s initial_hash)
 
 (** Free the hash accumulator *)
-val reclaim (#h:ehash_value_t) (s:ha)
+val reclaim (#h:hash_value_t) (s:ha)
   : STT unit
     (ha_val s h)
     (fun _ -> emp)
@@ -68,12 +65,12 @@ let maybe_aggregate_hashes (b:bool) (h0 h1: hash_value_t) =
   if b then aggregate_hashes h0 h1
   else h0
 
-val aggregate (#h1 #h2:ehash_value_t) (b1 b2: ha)
+val aggregate (#h1 #h2:hash_value_t) (b1 b2: ha)
   : STT bool
     (ha_val b1 h1 `star` ha_val b2 h2)
     (fun b -> ha_val b1 (maybe_aggregate_hashes b h1 h2) `star` ha_val b2 h2)
 
-val compare (#h1 #h2:ehash_value_t) (b1 b2:ha)
+val compare (#h1 #h2:hash_value_t) (b1 b2:ha)
   : ST bool
     (ha_val b1 h1 `star` ha_val b2 h2)
     (fun _ -> ha_val b1 h1 `star` ha_val b2 h2)
@@ -82,7 +79,7 @@ val compare (#h1 #h2:ehash_value_t) (b1 b2:ha)
       success <==> (h1 == h2))
   
 (** Hash the (input[0, l)) into the hash accumulate s *)
-val add (#h:ehash_value_t) (ha:ha)
+val add (#h:hash_value_t) (ha:ha)
         (#p:perm) 
         (#ivv:Ghost.erased (Seq.seq U8.t) { Seq.length ivv == iv_len })
         (#s:Ghost.erased (Seq.seq U8.t))
